Weidenbach_Book/IsaSAT_Propagate_Conflict.thy
@@ -131,76 +131,7 @@ lemma (in isasat_input_ops) unit_propagation_inner_loop_wl_loop_D_heur_alt_def:
       b
   }\<close>
   unfolding unit_propagation_inner_loop_wl_loop_D_heur_def Let_def zero_uint64_nat_def ..
-(*
-(* This bound absolutely not thight *)
-lemma unit_propagation_inner_loop_wl_loop_D_heur_inv_length_watchlist:
-  assumes \<open>unit_propagation_inner_loop_wl_loop_D_heur_inv S0 L (j, w, S)\<close> and
-    fast: \<open>isasat_fast S0\<close>
-  shows
-    \<open>length (get_watched_wl_heur S ! nat_of_lit L) \<le> uint64_max\<close> (is ?A) and
-    \<open>length (get_watched_wl_heur S ! nat_of_lit L) < uint64_max\<close> (is ?B) and
-    \<open>Suc w \<le> uint64_max\<close> (is ?C)
-proof -
-  obtain T where
-    ST: \<open>(S, T) \<in> twl_st_heur\<close> and
-    inner: \<open>unit_propagation_inner_loop_wl_loop_D_inv L (j, w, T)\<close> and
-    L: \<open>L \<in># \<L>\<^sub>a\<^sub>l\<^sub>l\<close> and
-    dom_eq: \<open>dom_m (get_clauses_wl_heur S) = dom_m (get_clauses_wl_heur S0)\<close>
-    using assms unfolding unit_propagation_inner_loop_wl_loop_D_heur_inv_def by blast
-  obtain U V where
-    corr_w: \<open>correct_watching_except j w L T\<close> and
-    lits_in: \<open>literals_are_\<L>\<^sub>i\<^sub>n T\<close> and
-    TU: \<open>(T, U) \<in> state_wl_l (Some (L, w))\<close> and
-    UV: \<open>(U, V) \<in> twl_st_l (Some L)\<close> and
-    struct_invs: \<open>twl_struct_invs V\<close> and
-    \<open>twl_stgy_invs V\<close> and
-    \<open>twl_list_invs U\<close> and
-    w_le: \<open>w \<le> length (watched_by T L)\<close>
-    using inner unfolding unit_propagation_inner_loop_wl_loop_D_inv_def
-     unit_propagation_inner_loop_wl_loop_inv_def
-     unit_propagation_inner_loop_l_inv_def
-     prod.case
-     by fast+
-  have alien: \<open>cdcl\<^sub>W_restart_mset.no_strange_atm (state\<^sub>W_of V)\<close>
-    using struct_invs unfolding twl_struct_invs_def cdcl\<^sub>W_restart_mset.cdcl\<^sub>W_all_struct_inv_def
-    by fast
-  have \<open>L \<in># all_lits_of_mm (mset `# ran_mf (get_clauses_wl T) + get_unit_clauses_wl T)\<close>
-    using lits_in L by (auto simp: image_image is_\<L>\<^sub>a\<^sub>l\<^sub>l_def literals_are_\<L>\<^sub>i\<^sub>n_def)
-  moreover have
-    \<open>set_mset (all_lits_of_mm (mset `# ran_mf (get_clauses_wl T) + get_unit_clauses_wl T)) =
-      set_mset (all_lits_of_mm (mset `# ran_mf (get_clauses_wl T) + get_unit_init_clss_wl T))\<close>
-    apply (subst all_clss_lf_ran_m[symmetric])+
-    apply (subst image_mset_union)+
-    using TU UV alien
-    by (cases T; cases U; cases V)
-      (auto simp: in_all_lits_of_mm_ain_atms_of_iff state_wl_l_def twl_st_l_def
-      cdcl\<^sub>W_restart_mset.no_strange_atm_def mset_take_mset_drop_mset')
-  ultimately have 1: \<open>fst `# mset ((get_watched_wl T) L) =
-      {#C \<in># dom_m (get_clauses_wl T). L \<in> set (watched_l ((get_clauses_wl T) \<propto> C))#}\<close>
-    using corr_w by (cases T)
-      (auto simp: correct_watching.simps clause_to_update_def all_lits_of_mm_union)
-  then have \<open>size (mset ((get_watched_wl T) L)) \<le> size (dom_m (get_clauses_wl T))\<close>
-    unfolding 1
-    by (cases T) (auto simp: correct_watching.simps clause_to_update_def)
-  moreover {
-    have \<open>Max_dom (get_clauses_wl T) \<le> uint_max\<close>
-      using fast ST
-      unfolding dom_eq[symmetric]
-      by (cases T)
-        (auto simp: twl_st_heur_def Max_dom_def dest!: multi_member_split)
-    then have \<open>size (dom_m (get_clauses_wl T)) < uint64_max\<close>
-      using fast ST size_dom_m_Max_dom[of \<open>get_clauses_wl T\<close>]
-      by (cases T)
-        (auto simp: twl_st_heur_def uint_max_def uint64_max_def)
-  }
-  ultimately have le_T: \<open>length ((get_watched_wl T) L) < uint64_max\<close>
-    by simp
-  moreover have \<open>length ((get_watched_wl T) L)  = length (get_watched_wl_heur S ! nat_of_lit L)\<close>
-    using L ST by (cases S; cases T) (auto simp: twl_st_heur_def map_fun_rel_def)
-  ultimately show ?A and ?B by simp_all
-  then show ?C
-    using w_le le_T by (cases T) auto
-qed *)
+
 
 sepref_register length_ll_fs_heur
 
@@ -321,17 +252,13 @@ sepref_thm select_and_remove_from_literals_to_update_wlfast_code
   unfolding select_and_remove_from_literals_to_update_wl_heur_alt_def isasat_bounded_assn_def
     one_uint32_nat_def[symmetric]
   supply [[goals_limit = 1]]
-       apply sepref_dbg_keep
-  apply sepref_dbg_trans_keep
-  apply sepref_dbg_trans_step_keep
-  apply sepref_dbg_side_unfold
   by sepref
 
 concrete_definition (in -) select_and_remove_from_literals_to_update_wlfast_code
    uses isasat_input_bounded_nempty.select_and_remove_from_literals_to_update_wlfast_code.refine_raw
    is \<open>(?f, _)\<in>_\<close>
 
-preparefast_code_thms (in -) select_and_remove_from_literals_to_update_wlfast_code_def
+prepare_code_thms (in -) select_and_remove_from_literals_to_update_wlfast_code_def
 
 lemmas select_and_remove_from_literals_to_update_wlfast_code_refine[sepref_fr_rules] =
    select_and_remove_from_literals_to_update_wlfast_code.refine[of \<A>\<^sub>i\<^sub>n,
@@ -365,6 +292,22 @@ prepare_code_thms (in -) literals_to_update_wl_literals_to_update_wl_empty_code_
 lemmas literals_to_update_wl_literals_to_update_wl_empty_code_hnr[sepref_fr_rules] =
    literals_to_update_wl_literals_to_update_wl_empty_code.refine[of \<A>\<^sub>i\<^sub>n, OF isasat_input_bounded_nempty_axioms]
 
+sepref_thm literals_to_update_wl_literals_to_update_wl_empty_fast_code
+  is \<open>RETURN o literals_to_update_wl_literals_to_update_wl_empty\<close>
+  :: \<open>isasat_bounded_assn\<^sup>k \<rightarrow>\<^sub>a bool_assn\<close>
+  unfolding literals_to_update_wl_literals_to_update_wl_empty_alt_def
+    isasat_bounded_assn_def
+  by sepref
+
+concrete_definition (in -) literals_to_update_wl_literals_to_update_wl_empty_fast_code
+   uses isasat_input_bounded_nempty.literals_to_update_wl_literals_to_update_wl_empty_fast_code.refine_raw
+   is \<open>(?f,_)\<in>_\<close>
+
+prepare_code_thms (in -) literals_to_update_wl_literals_to_update_wl_empty_fast_code_def
+
+lemmas literals_to_update_wl_literals_to_update_wl_empty_fast_code_hnr[sepref_fr_rules] =
+   literals_to_update_wl_literals_to_update_wl_empty_fast_code.refine[of \<A>\<^sub>i\<^sub>n, OF isasat_input_bounded_nempty_axioms]
+
 sepref_register literals_to_update_wl_literals_to_update_wl_empty
   select_and_remove_from_literals_to_update_wl_heur
   unit_propagation_inner_loop_wl_D_heur
@@ -387,28 +330,22 @@ prepare_code_thms (in -) unit_propagation_outer_loop_wl_D_def
 lemmas unit_propagation_outer_loop_wl_D[sepref_fr_rules] =
    unit_propagation_outer_loop_wl_D.refine[of \<A>\<^sub>i\<^sub>n, OF isasat_input_bounded_nempty_axioms]
 
-(* lemma unit_propagation_outer_loop_wl_D_fast_still_fast:
-  assumes
-    fast: \<open>\<forall>L\<in>#dom_m (get_clauses_wl_heur x). L < uint_max\<close> and
-    inv: \<open>unit_propagation_outer_loop_wl_D_heur_inv x s'\<close> and
-    le: \<open>RETURN (a1', a2') \<le> select_and_remove_from_literals_to_update_wl_heur s'\<close> and
-    L: \<open>L \<in># dom_m (get_clauses_wl_heur a1')\<close>
-  shows \<open>L < uint_max\<close>
-proof -
-  show ?thesis
-    using le fast L inv by (cases s')
-      (auto simp: select_and_remove_from_literals_to_update_wl_heur_def
-      unit_propagation_outer_loop_wl_D_heur_inv_def)
-qed *)
+lemma unit_propagation_outer_loop_wl_D_heur_fast:
+  \<open>length (get_clauses_wl_heur x) \<le> uint64_max \<Longrightarrow>
+       unit_propagation_outer_loop_wl_D_heur_inv x s' \<Longrightarrow>
+       length (get_clauses_wl_heur a1') =
+       length (get_clauses_wl_heur s') \<Longrightarrow>
+       (a, a2') \<in> unat_lit_rel \<Longrightarrow>
+       length (get_clauses_wl_heur s') \<le> uint64_max\<close>
+  by (auto simp: unit_propagation_outer_loop_wl_D_heur_inv_def)
 
-(*
 sepref_thm unit_propagation_outer_loop_wl_D_fast
   is \<open>PR_CONST unit_propagation_outer_loop_wl_D_heur\<close>
-  :: \<open>[isasat_fast]\<^sub>a isasat_bounded_assn\<^sup>d \<rightarrow> isasat_bounded_assn\<close>
-  supply [[goals_limit=1]] unit_propagation_outer_loop_wl_D_fast_still_fast[intro]
+  :: \<open>[\<lambda>S. length (get_clauses_wl_heur S) \<le> uint64_max]\<^sub>a isasat_bounded_assn\<^sup>d \<rightarrow> isasat_bounded_assn\<close>
+  supply [[goals_limit=1]] unit_propagation_outer_loop_wl_D_heur_fast[intro]
   apply (subst PR_CONST_def)
   unfolding unit_propagation_outer_loop_wl_D_heur_def
-    literals_to_update_wl_literals_to_update_wl_empty
+    literals_to_update_wl_literals_to_update_wl_empty_def[symmetric]
   by sepref
 
 concrete_definition (in -) unit_propagation_outer_loop_wl_D_fast
@@ -418,7 +355,7 @@ concrete_definition (in -) unit_propagation_outer_loop_wl_D_fast
 prepare_code_thms (in -) unit_propagation_outer_loop_wl_D_fast_def
 
 lemmas unit_propagation_outer_loop_wl_D_fast[sepref_fr_rules] =
-   unit_propagation_outer_loop_wl_D_fast.refine[of \<A>\<^sub>i\<^sub>n, OF isasat_input_bounded_nempty_axioms] *)
+   unit_propagation_outer_loop_wl_D_fast.refine[of \<A>\<^sub>i\<^sub>n, OF isasat_input_bounded_nempty_axioms]
 
 end
 
